Weidenbach_Book/CDCL_WNOT.thy
@@ -233,27 +233,27 @@ lemma skip_or_resolve_state_change:
     "\<exists>M. trail S = M @ trail T \<and> (\<forall>m \<in> set M. \<not>is_decided m)"
     "clauses S = clauses T"
     "backtrack_lvl S = backtrack_lvl T"
+    "init_clss S = init_clss T"
+    "learned_clss S = learned_clss T"
   using assms
 proof (induction rule: rtranclp_induct)
   case base
   case 1 show ?case by simp
   case 2 show ?case by simp
   case 3 show ?case by simp
+  case 4 show ?case by simp
+  case 5 show ?case by simp
 next
-  case (step T U) note st = this(1) and s_o_r = this(2) and IH = this(3) and IH' = this(3-5)
+  case (step T U) note st = this(1) and s_o_r = this(2) and IH = this(3) and IH' = this(3-)
 
   case 2 show ?case using IH' s_o_r by (auto elim!: rulesE simp: skip_or_resolve.simps)
-  case 3 show ?case using IH' s_o_r by (auto elim!: rulesE simp: skip_or_resolve.simps)
+  case 3 show ?case using IH' s_o_r by (cases \<open>trail T\<close>) (auto elim!: rulesE simp: skip_or_resolve.simps)
   case 1 show ?case
-    using s_o_r
-    proof cases
-      case s_or_r_skip
-      then show ?thesis using IH by (auto elim!: rulesE simp: skip_or_resolve.simps)
-    next
-      case s_or_r_resolve
-      then show ?thesis
-        using IH by (cases "trail T") (auto elim!: rulesE simp: skip_or_resolve.simps)
-    qed
+    using s_o_r IH by (cases "trail T") (auto elim!: rulesE simp: skip_or_resolve.simps)
+  case 4 show ?case
+    using s_o_r IH' by (cases "trail T") (auto elim!: rulesE simp: skip_or_resolve.simps)
+  case 5 show ?case
+    using s_o_r IH' by (cases "trail T") (auto elim!: rulesE simp: skip_or_resolve.simps)
 qed
 
 
@@ -270,12 +270,12 @@ lemma cdcl\<^sub>W_merge_is_cdcl\<^sub>N\<^sub>O\<^sub>T_merged_bj_learn:
   using cdcl\<^sub>W_restart inv
 proof induction
   case (fw_propagate S T) note propa = this(1)
-  then obtain M N U k L C where
-    H: "state_butlast S = (M, N, U, k, None)" and
+  then obtain M N U L C where
+    H: "state_butlast S = (M, N, U, None)" and
     CL: "C + {#L#} \<in># clauses S" and
     M_C: "M \<Turnstile>as CNot C" and
     undef: "undefined_lit (trail S) L" and
-    T: "state_butlast T = (Propagated L (C + {#L#}) # M, N, U, k, None)"
+    T: "state_butlast T = (Propagated L (C + {#L#}) # M, N, U, None)"
     by (auto elim: propagate_high_levelE)
   have "propagate\<^sub>N\<^sub>O\<^sub>T S T"
     using H CL T undef M_C by (auto simp: state_eq\<^sub>N\<^sub>O\<^sub>T_def clauses_def simp del: state_simp)
@@ -286,8 +286,7 @@ next
   then obtain L where
     undef_L: "undefined_lit (trail S) L" and
     atm_L: "atm_of L \<in> atms_of_mm (init_clss S)" and
-    T: "T \<sim> cons_trail (Decided L)
-      (update_backtrack_lvl (Suc (backtrack_lvl S)) S)"
+    T: "T \<sim> cons_trail (Decided L) S"
     by (auto elim: decideE)
   have "decide\<^sub>N\<^sub>O\<^sub>T S T"
     apply (rule decide\<^sub>N\<^sub>O\<^sub>T.decide\<^sub>N\<^sub>O\<^sub>T)
@@ -357,8 +356,7 @@ next
         U: "U \<sim> cons_trail (Propagated L D)
                  (reduce_trail_to M1
                       (add_learned_cls D
-                         (update_backtrack_lvl i
-                            (update_conflicting None T'))))"
+                        (update_conflicting None T')))"
         using bt by (auto elim: backtrackE)
       have [simp]: "clauses S = clauses T"
         using confl by (auto elim: rulesE)
@@ -912,7 +910,7 @@ next
     using full mono_rtranclp[of skip_or_resolve cdcl\<^sub>W_bj] unfolding full_def
     by (blast elim: skip_or_resolve.cases)
   moreover have "cdcl\<^sub>W_bj U V" and "no_step cdcl\<^sub>W_bj V"
-    using bt by (auto intro: cdcl\<^sub>W_bj.intros dest: backtrack_no_cdcl\<^sub>W_bj)
+    using bt by (auto dest: backtrack_no_cdcl\<^sub>W_bj)
   ultimately have "full1 cdcl\<^sub>W_bj T V"
     unfolding full1_def by auto
   then have "cdcl\<^sub>W_stgy\<^sup>*\<^sup>* T V"
@@ -1070,11 +1068,12 @@ proof -
         then show ?case by (simp add: f_0)
       next
         case (Suc k)
-        then show ?case
-          apply (cases \<open>k < j\<close>)
-            using f_s_o_r[of k] apply (auto simp: skip_or_resolve.simps elim!: rulesE)[]
-          using f_s_o_r[of "j - 1"] j_0
+        then have \<open>backtrack_lvl (f (Suc k)) = backtrack_lvl (f k)\<close>
+          apply (cases \<open>k < j\<close>; cases \<open>trail (f k)\<close>)
+            using f_s_o_r[of k] apply (auto simp: skip_or_resolve.simps elim!: rulesE)[2]
           by (auto simp: skip_or_resolve.simps elim!: rulesE simp del: local.state_simp)
+        then show ?case
+          using f_s_o_r[of k] Suc by simp
       qed
 
       have st_f: \<open>cdcl\<^sub>W_stgy\<^sup>*\<^sup>* ?T (f k)\<close> if \<open>k < j\<close> for k
@@ -1185,15 +1184,14 @@ proof -
     using conf by (auto elim: rulesE)
   have s_o_r: \<open>skip_or_resolve\<^sup>*\<^sup>* T U\<close>
     using full unfolding full_def by blast
-  moreover have \<open>\<exists>Ma. M @ trail y = Ma @ tl (trail y)\<close> for M y
-    by (cases \<open>trail y\<close>) auto
-  ultimately have
+  then have
     \<open>\<exists>M. trail T = M @ trail U\<close> and
     bt_T_U: \<open>backtrack_lvl T = backtrack_lvl U\<close> and
-    init_clss_T_U: \<open>init_clss T = init_clss U\<close> and
-    learned_clss_T_U: \<open>learned_clss T = learned_clss U\<close> and
-    clss_T_U: \<open>clauses T = clauses U\<close>
-    by (induction rule: rtranclp_induct) (auto simp: skip_or_resolve.simps elim!: rulesE)
+    bt_lvl_T_U: \<open>backtrack_lvl T = backtrack_lvl U\<close> and
+    clss_T_U: \<open>clauses T = clauses U\<close> and
+    init_T_U: \<open>init_clss T = init_clss U\<close> and
+    learned_T_U: \<open>learned_clss T = learned_clss U\<close>
+    using skip_or_resolve_state_change[of T U] by blast+
   then obtain M where M: \<open>trail T = M @ trail U\<close>
     by blast
   obtain D :: "'v literal multiset" and K L :: "'v literal"  and
@@ -1208,8 +1206,7 @@ proof -
     V: "V \<sim> cons_trail (Propagated L D)
         (reduce_trail_to M1
           (add_learned_cls D
-            (update_backtrack_lvl i
-              (update_conflicting None U))))"
+            (update_conflicting None U)))"
     using bt by (auto elim!: rulesE)
   obtain M' where M': \<open>trail U = M' @ M2 @ Decided K # M1\<close>
     using decomp by auto
@@ -1231,7 +1228,7 @@ proof -
   have \<open>atm_of L \<in> atms_of_mm (init_clss V)\<close>
     using inv_V V decomp unfolding cdcl\<^sub>W_all_struct_inv_def no_strange_atm_def by auto
   moreover have init_clss_V_S: \<open>init_clss V = init_clss S\<close>
-    using T V init_clss_T_U by auto
+    using T V init_T_U by auto
   ultimately have atm_L: \<open>atm_of L \<in> atms_of_mm (clauses S)\<close>
     by (auto simp: clauses_def)
 
@@ -1282,8 +1279,7 @@ lemma cdcl\<^sub>W_with_strategy_propagate\<^sub>N\<^sub>O\<^sub>T_propagate_iff
   \<open>cdcl\<^sub>W_with_strategy.propagate\<^sub>N\<^sub>O\<^sub>T S T \<longleftrightarrow> propagate S T\<close> (is "?NOT \<longleftrightarrow> ?W")
 proof (rule iffI)
   assume ?NOT
-  then show ?W
-    by (auto elim!: cdcl\<^sub>W_with_strategy.propagate\<^sub>N\<^sub>O\<^sub>TE)[]
+  then show ?W by auto
 next
   assume ?W
   then obtain E L where
@@ -1392,17 +1388,17 @@ next
     have atm: \<open>atms_of_mm (clauses S) = atms_of_mm (init_clss S)\<close>
       using 3(3) unfolding cdcl\<^sub>W_all_struct_inv_def no_strange_atm_def
       by (auto simp: clauses_def)
-    have \<open>decide S (cons_trail (Decided L) (update_backtrack_lvl (Suc (backtrack_lvl S)) S))\<close>
+    have \<open>decide S (cons_trail (Decided L) S)\<close>
       apply (rule decide_rule)
       using 3 by (auto simp: atm)
-  moreover have \<open>cons_trail (Decided L) (update_backtrack_lvl (Suc (backtrack_lvl S)) S) \<sim>\<^sub>N\<^sub>O\<^sub>T
+  moreover have \<open>cons_trail (Decided L) S \<sim>\<^sub>N\<^sub>O\<^sub>T
     cons_trail (Decided L) S\<close>
     by (simp add: state_eq\<^sub>N\<^sub>O\<^sub>T_def del: state_simp)
   ultimately show "\<exists>T. cdcl\<^sub>W_with_strategy.decide\<^sub>N\<^sub>O\<^sub>T S T \<or>
     cdcl\<^sub>W_with_strategy.propagate\<^sub>N\<^sub>O\<^sub>T S T \<or>
     cdcl\<^sub>W_with_strategy.backjump_l S T"
     using cdcl\<^sub>W_with_strategy.decide\<^sub>N\<^sub>O\<^sub>T.intros[of S L
-        "cons_trail (Decided L) (update_backtrack_lvl (Suc (backtrack_lvl S)) S)"]
+        "cons_trail (Decided L) S"]
     apply auto
     done
 qed
