Weidenbach_Book/CDCL_W_Optimal_Model.thy
@@ -7,9 +7,9 @@ locale conflict_driven_clause_learning_with_adding_init_clause_cost\<^sub>W_no_s
     state_eq state
     \<comment> \<open>functions for the state: \<close>
       \<comment> \<open>access functions:\<close>
-    trail init_clss learned_clss backtrack_lvl conflicting
+    trail init_clss learned_clss conflicting
       \<comment> \<open>changing state:\<close>
-    cons_trail tl_trail add_learned_cls remove_cls update_backtrack_lvl
+    cons_trail tl_trail add_learned_cls remove_cls
     update_conflicting
 
       \<comment> \<open>get state:\<close>
@@ -18,19 +18,17 @@ locale conflict_driven_clause_learning_with_adding_init_clause_cost\<^sub>W_no_s
     add_init_cls
   for
     state_eq :: "'st \<Rightarrow> 'st \<Rightarrow> bool" (infix "\<sim>" 50) and
-    state :: "'st \<Rightarrow> ('v, 'v clause) ann_lits \<times> 'v clauses \<times> 'v clauses \<times> nat \<times> 'v clause option \<times>
+    state :: "'st \<Rightarrow> ('v, 'v clause) ann_lits \<times> 'v clauses \<times> 'v clauses \<times> 'v clause option \<times>
       'a \<times> 'b" and
     trail :: "'st \<Rightarrow> ('v, 'v clause) ann_lits" and
     init_clss :: "'st \<Rightarrow> 'v clauses" and
     learned_clss :: "'st \<Rightarrow> 'v clauses" and
-    backtrack_lvl :: "'st \<Rightarrow> nat" and
     conflicting :: "'st \<Rightarrow> 'v clause option" and
 
     cons_trail :: "('v, 'v clause) ann_lit \<Rightarrow> 'st \<Rightarrow> 'st" and
     tl_trail :: "'st \<Rightarrow> 'st" and
     add_learned_cls :: "'v clause \<Rightarrow> 'st \<Rightarrow> 'st" and
     remove_cls :: "'v clause \<Rightarrow> 'st \<Rightarrow> 'st" and
-    update_backtrack_lvl :: "nat \<Rightarrow> 'st \<Rightarrow> 'st" and
     update_conflicting :: "'v clause option \<Rightarrow> 'st \<Rightarrow> 'st" and
 
     init_state :: "'v clauses \<Rightarrow> 'st" and
@@ -46,7 +44,7 @@ locale conflict_driven_clause_learning_with_adding_init_clause_cost\<^sub>W_no_s
 begin
 
 definition additional_info' :: "'st \<Rightarrow> 'b" where
-"additional_info' S = (\<lambda>(_, _, _, _, _, _, D). D) (state S)"
+"additional_info' S = (\<lambda>(_, _, _, _, _, D). D) (state S)"
 
 end
   
@@ -55,9 +53,9 @@ locale conflict_driven_clause_learning_with_adding_init_clause_cost\<^sub>W_ops 
     state_eq state
     \<comment> \<open>functions for the state: \<close>
       \<comment> \<open>access functions:\<close>
-    trail init_clss learned_clss backtrack_lvl conflicting
+    trail init_clss learned_clss conflicting
       \<comment> \<open>changing state:\<close>
-    cons_trail tl_trail add_learned_cls remove_cls update_backtrack_lvl
+    cons_trail tl_trail add_learned_cls remove_cls
     update_conflicting
 
       \<comment> \<open>get state:\<close>
@@ -66,19 +64,17 @@ locale conflict_driven_clause_learning_with_adding_init_clause_cost\<^sub>W_ops 
     add_init_cls add_additional_information conflicting_clauses weight
   for
     state_eq :: "'st \<Rightarrow> 'st \<Rightarrow> bool" (infix "\<sim>" 50) and
-    state :: "'st \<Rightarrow> ('v, 'v clause) ann_lits \<times> 'v clauses \<times> 'v clauses \<times> nat \<times> 'v clause option \<times>
+    state :: "'st \<Rightarrow> ('v, 'v clause) ann_lits \<times> 'v clauses \<times> 'v clauses \<times>  'v clause option \<times>
       'a \<times> 'b" and
     trail :: "'st \<Rightarrow> ('v, 'v clause) ann_lits" and
     init_clss :: "'st \<Rightarrow> 'v clauses" and
     learned_clss :: "'st \<Rightarrow> 'v clauses" and
-    backtrack_lvl :: "'st \<Rightarrow> nat" and
     conflicting :: "'st \<Rightarrow> 'v clause option" and
 
     cons_trail :: "('v, 'v clause) ann_lit \<Rightarrow> 'st \<Rightarrow> 'st" and
     tl_trail :: "'st \<Rightarrow> 'st" and
     add_learned_cls :: "'v clause \<Rightarrow> 'st \<Rightarrow> 'st" and
     remove_cls :: "'v clause \<Rightarrow> 'st \<Rightarrow> 'st" and
-    update_backtrack_lvl :: "nat \<Rightarrow> 'st \<Rightarrow> 'st" and
     update_conflicting :: "'v clause option \<Rightarrow> 'st \<Rightarrow> 'st" and
 
     init_state :: "'v clauses \<Rightarrow> 'st" and
@@ -88,8 +84,7 @@ locale conflict_driven_clause_learning_with_adding_init_clause_cost\<^sub>W_ops 
     weight :: \<open>'st \<Rightarrow> 'a\<close> +
   assumes
     state_prop[simp]:
-      \<open>state S = (trail S, init_clss S, learned_clss S, backtrack_lvl S,
-      conflicting S, weight S, additional_info' S)\<close> 
+      \<open>state S = (trail S, init_clss S, learned_clss S, conflicting S, weight S, additional_info' S)\<close>  
 begin
 
 sublocale conflict_driven_clause_learning_with_adding_init_clause\<^sub>W
@@ -122,7 +117,6 @@ inductive improve :: "'st \<Rightarrow> 'st \<Rightarrow> bool" where
   M \<Turnstile>asm init_clss S \<Longrightarrow>
   T \<sim> update_conflicting (Some (negate_trail S)) S \<Longrightarrow> 
   improve S (add_additional_information S)"
-
 
 end
 end
