Weidenbach_Book/CDCL_W_Restart.thy
@@ -9,28 +9,26 @@ locale cdcl\<^sub>W_restart_restart =
     state
     \<comment> \<open>functions for the state: \<close>
       \<comment> \<open>access functions:\<close>
-    trail init_clss learned_clss backtrack_lvl conflicting
+    trail init_clss learned_clss conflicting
       \<comment> \<open>changing state:\<close>
-    cons_trail tl_trail add_learned_cls remove_cls update_backtrack_lvl
+    cons_trail tl_trail add_learned_cls remove_cls
     update_conflicting
 
       \<comment> \<open>get state:\<close>
     init_state
   for
     state_eq :: "'st \<Rightarrow> 'st \<Rightarrow> bool" (infix "\<sim>" 50) and
-    state :: "'st \<Rightarrow> ('v, 'v clause) ann_lits \<times> 'v clauses \<times> 'v clauses \<times> nat \<times> 'v clause option \<times>
+    state :: "'st \<Rightarrow> ('v, 'v clause) ann_lits \<times> 'v clauses \<times> 'v clauses \<times> 'v clause option \<times>
       'b" and
     trail :: "'st \<Rightarrow> ('v, 'v clause) ann_lits" and
     init_clss :: "'st \<Rightarrow> 'v clauses" and
     learned_clss :: "'st \<Rightarrow> 'v clauses" and
-    backtrack_lvl :: "'st \<Rightarrow> nat" and
     conflicting :: "'st \<Rightarrow> 'v clause option" and
 
     cons_trail :: "('v, 'v clause) ann_lit \<Rightarrow> 'st \<Rightarrow> 'st" and
     tl_trail :: "'st \<Rightarrow> 'st" and
     add_learned_cls :: "'v clause \<Rightarrow> 'st \<Rightarrow> 'st" and
     remove_cls :: "'v clause \<Rightarrow> 'st \<Rightarrow> 'st" and
-    update_backtrack_lvl :: "nat \<Rightarrow> 'st \<Rightarrow> 'st" and
     update_conflicting :: "'v clause option \<Rightarrow> 'st \<Rightarrow> 'st" and
 
     init_state :: "'v clauses \<Rightarrow> 'st" +
@@ -542,9 +540,9 @@ locale luby_sequence_restart =
     \<comment> \<open>functions for the state: \<close>
     state_eq state
       \<comment> \<open>access functions:\<close>
-    trail init_clss learned_clss backtrack_lvl conflicting
+    trail init_clss learned_clss conflicting
       \<comment> \<open>changing state:\<close>
-    cons_trail tl_trail add_learned_cls remove_cls update_backtrack_lvl
+    cons_trail tl_trail add_learned_cls remove_cls
     update_conflicting
 
       \<comment> \<open>get state:\<close>
@@ -552,20 +550,18 @@ locale luby_sequence_restart =
   for
     ur :: nat and
     state_eq :: "'st \<Rightarrow> 'st \<Rightarrow> bool" (infix "\<sim>" 50) and
-    state :: "'st \<Rightarrow> ('v, 'v clause) ann_lits \<times> 'v clauses \<times> 'v clauses \<times> nat \<times> 'v clause option \<times>
+    state :: "'st \<Rightarrow> ('v, 'v clause) ann_lits \<times> 'v clauses \<times> 'v clauses \<times> 'v clause option \<times>
       'b" and
     trail :: "'st \<Rightarrow> ('v, 'v clause) ann_lits" and
     hd_trail :: "'st \<Rightarrow> ('v, 'v clause) ann_lit" and
     init_clss :: "'st \<Rightarrow> 'v clauses" and
     learned_clss :: "'st \<Rightarrow> 'v clauses" and
-    backtrack_lvl :: "'st \<Rightarrow> nat" and
     conflicting :: "'st \<Rightarrow> 'v clause option" and
 
     cons_trail :: "('v, 'v clause) ann_lit \<Rightarrow> 'st \<Rightarrow> 'st" and
     tl_trail :: "'st \<Rightarrow> 'st" and
     add_learned_cls :: "'v clause \<Rightarrow> 'st \<Rightarrow> 'st" and
     remove_cls :: "'v clause \<Rightarrow> 'st \<Rightarrow> 'st" and
-    update_backtrack_lvl :: "nat \<Rightarrow> 'st \<Rightarrow> 'st" and
     update_conflicting :: "'v clause option \<Rightarrow> 'st \<Rightarrow> 'st" and
 
     init_state :: "'v clauses \<Rightarrow> 'st"
